\documentclass[../main.tex]{subfiles}

\pagestyle{main}
\renewcommand{\chaptermark}[1]{\markboth{\chaptername\ \thechapter}{}}
\setcounter{chapter}{7}

\begin{document}




\chapter{Intervals}\label{sct:8}
\section{Journal}
\marginnote{2/9:}Now that we have constructed $\R$ and proved the fundamental facts about it, we will work with the real numbers $\R$ instead of an arbitrary continuum $C$. We will leave behind Dedekind cuts and think of elements of $\R$ as numbers. Accordingly, from now on, we will use lower-case letters like $x$ for real numbers and will write $+$ and $\cdot$ for $\oplus$ and $\otimes$. We will also now use the standard notation $(a,b)$ for the region $\underline{ab}=\{x\in\R\mid a<x<b\}$. Even though the notation is the same, this is \emph{not} the same object as the ordered pair $(a,b)$.\par
More generally, we adopt the following standard notation:
\begin{align}
    \begin{split}
        (a,b) &= \{x\in\R\mid a<x<b\}\\
        [a,b) &= \{x\in\R\mid a\leq x<b\}\\
        (a,b] &= \{x\in\R\mid a<x\leq b\}\\
        [a,b] &= \{x\in\R\mid a\leq x\leq b\}\\
        (a,\infty) &= \{x\in\R\mid a<x\}\\
        [a,\infty) &= \{x\in\R\mid a\leq x\}\\
        (-\infty,b) &= \{x\in\R\mid x<b\}\\
        (-\infty,b] &= \{x\in\R\mid x\leq b\}
    \end{split}\label{eqn:8.1}
\end{align}

\begin{exercise}\label{exr:8.1}
    Identify the sets in Equations \ref{eqn:8.1} that are open/closed/neither.
    \begin{proof}
        Note that by Theorem \ref{trm:5.1}, any of these sets proven to be just one of open or closed will not be the other, i.e., a set proven to be open will not be closed and vice versa.\par\smallskip
        By Corollary \ref{cly:4.11}, $(a,b)$ is open.\par
        By an adaptation of Corollary \ref{cly:5.14}, $b\in LP([a,b))$ but $b\notin[a,b)$. Since $[a,b)$ doesn't contain all of its limit points, Definition \ref{dfn:4.1} tells us that it is not closed. Additionally, since $a\in LP(C\setminus[a,b))$ but $a\notin C\setminus[a,b)$, Definition \ref{dfn:4.8} tells us that it is not open. Therefore, it is neither.\par
        The proof that $(a,b]$ is neither is symmetric to the previous case.\par
        By Corollaries \ref{cly:5.15} and \ref{cly:4.7}, $[a,b]$ is closed.\par
        By Corollary \ref{cly:4.13}, $(a,\infty)$ is open.\par
        By Corollary \ref{cly:4.13} and Definition \ref{dfn:4.8}, $[a,\infty)=C\setminus(-\infty,a)$ is closed.\par
        The proofs that $(-\infty,b)$ and $(-\infty,b]$ are open and closed, respectively, are symmetric to the previous two cases, respectively.
    \end{proof}
\end{exercise}

\begin{definition}\label{dfn:8.2}
    A set $I\subset\R$ is an \textbf{interval} if for all $x,y\in I$ with $x<y$, $[x,y]\subset I$.
\end{definition}
\pagebreak

\begin{lemma}\label{lem:8.3}
    A proper subset $I\subsetneq\R$ is an interval if and only if it takes one of the eight forms in Equations \ref{eqn:8.1}.
    \begin{proof}
        Suppose first that $I\subsetneq\R$ is an interval. If $I=\emptyset$, then $I=(a,a)$ for any $a\in\R$, and we are done. Thus, we will assume for the remainder of the proof of the forward direction that $I$ is nonempty. To address this case, we will first prove that the facts that $I\subsetneq\R$, $I\neq\emptyset$, and $I$ is an interval imply that $I$ is bounded above, bounded below, or both. Then in each of these three cases, we will look at whether $\sup I$ and $\inf I$ (if they exist) are elements of the set or not to differentiate between the eight forms in Equations \ref{eqn:8.1}. Let's begin.\par\medskip
        Suppose for the sake of contradiction that there exists a nonempty interval $I\subsetneq\R$ that is neither bounded above nor bounded below. Since $I\subsetneq\R$, we have by Definition \ref{dfn:1.3} that there exists a point $p\in\R$ such that $p\notin I$. Additionally, since $I$ is neither bounded above nor below, Definition \ref{dfn:5.6} implies that $p$ is neither an upper nor a lower bound on $I$. Thus, there exist $x,y\in I$ such that $x<p$ and $y>p$. Now by Definition \ref{dfn:8.2}, $[x,y]\subset I$. But it follows by Definition \ref{dfn:1.3} that every point in $[x,y]$, including $p$, is an element of $I$, a contradiction.\par\medskip
        We now divide into three cases ($I$ is exclusively bounded below, $I$ is exclusively bounded above, and $I$ is bounded both below and above).\par\smallskip
        First, suppose that $I$ is only bounded below. Since $I$ is a nonempty subset of $\R$ that is bounded below, we have by Theorem \ref{trm:5.17} that $\inf I$ exists. We divide into two cases again ($\inf I\in I$ and $\inf I\notin I$).\par
        If $\inf I\in I$, then we can demonstrate that $I=[\inf I,\infty)$. To do this, Definition \ref{dfn:1.2} tells us that it will suffice to verify that every $p\in I$ is an element of $[\inf I,\infty)$ and vice versa. Let $p$ be an arbitrary element of $I$. Then $p\in\R$ and by Definitions \ref{dfn:5.7} and \ref{dfn:5.6}, $\inf I\leq p$. Therefore, $p\in[\inf I,\infty)$, as desired. Now let $p$ be an arbitrary element of $[\inf I,\infty)$. Then $\inf I\leq p$. Additionally, since $I$ is not bounded above, we have by Definition \ref{dfn:5.6} that there exists $y\in I$ such that $y>p$. Since $\inf I\in I$, $y\in I$, and $\inf I<y$ (by transitivity), $[\inf I,y]\subset I$ by Definition \ref{dfn:8.2}. This combined with the fact that $p\in[\inf I,y]$ (we know that $\inf I\leq p<y$, so $\inf I\leq p\leq y$) implies that $p\in I$, as desired.\par
        If $\inf I\notin I$, then we can demonstrate that $I=(\inf I,\infty)$. As before, to do so, it will suffice to verify that every $p\in I$ is an element of $(\inf I,\infty)$ and vice versa. Let $p$ be an arbitrary element of $I$. Then $p\in\R$ and by Definitions \ref{dfn:5.7} and \ref{dfn:5.6}, $\inf I\leq p$. The additional constraint that $\inf I\notin I$ implies that $\inf I<p$. Therefore, $p\in(\inf I,\infty)$, as desired. Now let $p$ be an arbitrary element of $(\inf I,\infty)$. Then $\inf I<p$. It follows by Lemma \ref{lem:5.11} that there exists a $z\in I$ such that $\inf I\leq z<p$. Additionally, since $I$ is not bounded above, we have by Definition \ref{dfn:5.6} that there exists $y\in I$ such that $y>p$. Since $z\in I$, $y\in I$, and $z<y$ (by transitivity), $[z,y]\subset I$ by Definition \ref{dfn:8.2}. This combined with the fact that $p\in[z,y]$ (we know that $z<p<y$, so $z\leq p\leq y$) implies that $p\in I$, as desired.\par\smallskip
        Second, suppose that $I$ is only bounded above. The proof of this case is symmetric to that of the first.\par\smallskip
        Third, suppose that $I$ is bounded below and above. Since $I$ is a nonempty subset of $\R$ that is bounded above and below, we have by consecutive applications of Theorem \ref{trm:5.17} that both $\sup I$ and $\inf I$ exist. We divide into four cases ($\inf I\in I$ and $\sup I\in I$, $\inf I\in I$ and $\sup I\notin I$, $\inf I\notin I$ and $\sup I\in I$, and $\inf I\notin I$ and $\sup I\notin I$).\par
        If $\inf I\in I$ and $\sup I\in I$, then we can demonstrate that $I=[\inf I,\sup I]$. We divide into two cases again ($\inf I=\sup I$ and $\inf I\neq\sup I$). If $\inf I=\sup I\in I$, then $I=\{\inf I\}=\{\sup I\}=[\inf I,\sup I]$, as desired. On the other hand, if $\inf I\neq\sup I$, we continue. To demonstrate that $I=[\inf I,\sup I]$, Theorem \ref{trm:1.7} tells us that it will suffice to verify that $I\subset[\inf I,\sup I]$ and $[\inf I,\sup I]\subset I$. To verify that the former claim, Definition \ref{dfn:1.3} tells us that it will suffice to confirm that every $p\in I$ is an element of $[\inf I,\sup I]$. Let $p$ be an arbitrary element of $I$. Then $p\in\R$ and by consecutive applications of Definitions \ref{dfn:5.7} and \ref{dfn:5.6}, $\inf I\leq p$ and $p\leq\sup I$. Therefore, $p\in[\inf I,\sup I]$, as desired. On the other hand, since $\inf I\in I$, $\sup I\in I$, and $\inf I<\sup I$ (as follows from Definition \ref{dfn:5.7} and the fact that they are unequal), $[\inf I,\sup I]\subset I$ by Definition \ref{dfn:8.2}, as desired.\par
        If $\inf I\in I$ and $\sup I\notin I$, then we can demonstrate that $I=[\inf I,\sup I)$. To do so, it will suffice to verify that every $p\in I$ is an element of $[\inf I,\sup I)$ and vice versa. Let $p$ be an arbitrary element of $I$. Then $p\in\R$ and by Definitions \ref{dfn:5.7} and \ref{dfn:5.6}, $\inf I\leq p$ and $p\leq \sup I$. The additional constraint that $\sup I\notin I$ implies that $p<\sup I$. Therefore, $p\in[\inf I,\sup I)$, as desired. Now let $p$ be an arbitrary element of $[\inf I,\sup I)$. Then $\inf I\leq p<\sup I$. It follows by Lemma \ref{lem:5.11} that there exists a $y\in I$ such that $p<y\leq\sup I$. Since $\inf I\in I$, $y\in I$, and $\inf I<y$ (by transitivity), $[\inf I,y]\subset I$ by Definition \ref{dfn:8.2}. This combined with the fact that $p\in[\inf I,y]$ (we know that $\inf I\leq p<y$, so $\inf I\leq p\leq y$) implies that $p\in I$, as desired.\par
        If $\inf I\notin I$ and $\sup I\in I$, the proof is symmetric to that of the previous case.\par
        If $\inf I\notin I$ and $\sup I\notin I$, then we can demonstrate that $I=(\inf I,\sup I)$. To do so, it will suffice to verify that every $p\in I$ is an element of $(\inf I,\sup I)$ and vice versa. Let $p$ be an arbitrary element of $I$. Then $p\in\R$ and by Definitions \ref{dfn:5.7} and \ref{dfn:5.6}, $\inf I\leq p$ and $p\leq \sup I$. The additional constraints that $\inf I\notin I$ and $\sup I\notin I$ imply that $\inf I<p$ and $p<\sup I$, respectively. Therefore, $p\in(\inf I,\sup I)$, as desired. Now let $p$ be an arbitrary element of $(\inf I,\sup I)$. Then $\inf I<p<\sup I$. It follows by consecutive applications of Lemma \ref{lem:5.11} that there exist $x,y\in I$ such that $\inf I\leq x<p$ and $p<y\leq\sup I$. Since $x\in I$, $y\in I$, and $x<y$ (by transitivity), $[x,y]\subset I$ by Definition \ref{dfn:8.2}. This combined with the fact that $p\in[x,y]$ (we know that $x<p<y$, so $x\leq p\leq y$) implies that $p\in I$, as desired.\par\bigskip
        Now suppose that $I\subsetneq\R$ takes one of the eight forms in Equations \ref{eqn:8.1}. To prove that $I$ is an interval, Definition \ref{dfn:8.2} tells us that it will suffice to show that for all $x,y\in I$ with $x<y$, $[x,y]\subset I$. Let $x,y$ be arbitrary elements of $I$ with $x<y$. We divide into eight cases (one for each equation in Equations \ref{eqn:8.1}).\par\smallskip
        First, suppose that $I=(a,b)$. To demonstrate that $[x,y]\subset I$, Definition \ref{dfn:1.3} tells us that it will suffice to confirm that every $z\in[x,y]$ is an element of $I$. Let $z$ be an arbitrary element of $[x,y]$. Then by Corollary \ref{cly:5.15}, $x\leq z\leq y$. But since $a<x<y<b$ by Equations \ref{eqn:8.1}, the fact that $a<x\leq z\leq y<b$ implies by Equations \ref{eqn:8.1} that $z\in(a,b)$, as desired.\par
        The proofs of the second, third, and fourth equations are symmetric to that of the first.\par
        Fifth, suppose that $I=(a,\infty)$. To demonstrate that $[x,y]\subset I$, Definition \ref{dfn:1.3} tells us that it will suffice to confirm that every $z\in[x,y]$ is an element of $I$. Let $z$ be an arbitrary element of $[x,y]$. Then by Corollary \ref{cly:5.15}, $x\leq z\leq y$. But since $a<x$ by Equations \ref{eqn:8.1}, the fact that $a<x\leq z$ implies by Equations \ref{eqn:8.1} that $z\in(a,\infty)$, as desired.\par
        The proofs of the sixth, seventh, and eighth equations are symmetric to that of the first.
    \end{proof}
\end{lemma}

\begin{definition}\label{dfn:8.4}
    The \textbf{absolute value} of a real number $x$ is the non-negative number $|x|$ defined by
    \begin{equation*}
        |x| =
        \begin{cases}
            x & x\geq 0\\
            -x & x<0
        \end{cases}
    \end{equation*}
\end{definition}

\begin{exercise}\label{exr:8.5}
    Show that $|x|=|-x|$ for all $x\in\R$. (Note that this also means that $|x-y|=|y-x|$ for any $x,y\in\R$.)
    \begin{proof}
        Let $x$ be an arbitrary element of $\R$. We divide into three cases ($x=0$, $x>0$, and $x<0$). First, suppose that $x=0$. Then since $0=-0$, clearly $|0|=|-0|$, as desired. Second, suppose that $x>0$. Then by Lemma \ref{lem:7.23}\footnote{And, technically, Theorem 7.47.} $-x<0$. Thus, by consecutive applications of Definition \ref{dfn:8.4}, $|x|=x$ and $|-x|=-(-x)$. Therefore, since $-(-x)=x$ by Corollary \ref{cly:7.11}, $|x|=x=|-x|$, as desired. Third, suppose that $x<0$. Then by Lemma \ref{lem:7.23}, $-x>0$. Thus, by consecutive applications of Definition \ref{dfn:8.4}, $|x|=-x$ and $|-x|=-x$. Therefore, $|x|=-x=|-x|$, as desired.
    \end{proof}
\end{exercise}

\begin{definition}\label{dfn:8.6}
    The \textbf{distance} between $x\in\R$ and $y\in\R$ is defined to be $|x-y|$.
\end{definition}

\begin{remark}\label{rmk:8.7}
    It follows from Definition \ref{dfn:8.6} that $|x|$ is the distance between $x$ and $0$.
\end{remark}

\begin{lemma}\label{lem:8.8}
    For any real numbers $x,y,z$, we have
    \begin{enumerate}[label={\textup{(}\alph*\textup{)}}]
        \item $|x+y|\leq|x|+|y|$.
        \item $|x-z|\leq|x-y|+|y-z|$.
        \item $||x|-|y||\leq|x-y|$.
    \end{enumerate}
    \begin{proof}[Proof of a]
        We divide into four cases ($x\geq 0$ and $y\geq 0$, $x\geq 0$ and $y<0$, $x<0$ and $y\geq 0$, and $x<0$ and $y<0$).\par
        First, suppose that $x\geq 0$ and $y\geq 0$. Then by Definition \ref{dfn:7.21}, $x+y\geq 0$. Thus, by consecutive applications of Definition \ref{dfn:8.4}, $|x+y|=x+y$, $|x|=x$, and $|y|=y$. Therefore, $|x+y|=x+y\leq x+y=|x|+|y|$, as desired.\par
        Second, suppose that $x\geq 0$ and $y<0$. By Definition \ref{dfn:8.4}, $|x|=x$ and $|y|=-y$. We now divide into two cases ($x+y\geq 0$ and $x+y<0$). If $x+y\geq 0$, then $|x+y|=x+y$. Additionally, since $y<0$, Lemma \ref{lem:7.23} implies that $0<-y$. Consequently, by transitivity, $y<-y=|y|$. It follows by Definition \ref{dfn:7.21} that $x+y<x+|y|$. Therefore, $|x+y|=x+y<x+|y|=|x|+|y|$, so $|x+y|\leq|x|+|y|$, as desired. On the other hand, if $x+y<0$, then $|x+y|=-(x+y)=-x+(-y)=-x+|y|$. Additionally, by Lemma \ref{lem:7.23}, $x\geq 0$ implies that $-x\leq 0$. It follows by Definition \ref{dfn:7.21} since $-x\leq x$ that $-x+|y|\leq x+|y|$. Therefore, $|x+y|=-x+|y|\leq x+|y|=|x|+|y|$, as desired.\par
        The proof of the third case is symmetric to that of the second.\par
        The proof of the fourth case is symmetric to that of the first.
    \end{proof}
    \begin{proof}[Proof of b]
        By part (a), $|x-z|=|x-y+y-z|\leq |x-y|+|y-z|$, as desired.
    \end{proof}
    \begin{proof}[Proof of c]
        To prove that $||x|-|y||\leq|x-y|$, Definition \ref{dfn:8.4} tells us that it will suffice to show that $|x|-|y|\leq|x-y|$ and $-(|x|-|y|)\leq|x-y$. By part (a), $|x|=|x-y+y|\leq|x-y|+|y|$, so $|x|-|y|\leq|x-y|$. Similarly, $|y|-|x|\leq|x-y|$, so $-(|x|-|y|)\leq|x-y|$, as desired.
    \end{proof}
\end{lemma}

\begin{exercise}\label{exr:8.9}
    Let $a,\delta\in\R$ with $\delta>0$. Prove that
    \begin{equation*}
        (a-\delta,a+\delta) = \{x\in\R\mid|x-a|<\delta\}
    \end{equation*}
    \begin{lemma*}
        For any $a,b\in\R$ such that $0<b$, $|a|<b$ if and only if $-b<a<b$.
        \begin{proof}
            Suppose first that $|a|<b$. We divide into two cases ($a\geq 0$ and $a<0$). If $a\geq 0$, then by Definition \ref{dfn:8.4}, $0\leq a=|a|<b$. Additionally, by Lemma \ref{lem:7.23}, $-b<0$. Therefore, $-b<0\leq a<b$, as desired. If $a<0$, then by Definition \ref{dfn:8.4}, $-a=|a|<b$. It follows by Definition \ref{dfn:7.21} (by adding $a-b$ to both sides) that $-b<a$. Additionally, by Lemma \ref{lem:7.23}, $a<0$ implies $0<-a$, so we know that $a<-a$. Therefore, $-b<a<-a<b$, as desired.\par
            Now suppose that $-b<a<b$. We divide into two cases ($a\geq 0$ and $a>0$). If $a\geq 0$, then by Definition \ref{dfn:8.4}, $|a|=a<b$, as desired. If $a<0$, then by Definition \ref{dfn:8.4}, $|a|=-a$. Since $-b<a$, Definition \ref{dfn:7.21} implies (by adding $b-a$ to both sides) that $-a<b$. Therefore, $|a|=-a<b$, as desired.
        \end{proof}
    \end{lemma*}
    \begin{proof}[Proof of Exercise \ref{exr:8.9}]
        To prove that $(a-\delta,a+\delta)=\{x\in\R\mid|x-a|<\delta\}$, Definition \ref{dfn:1.2} tells us that it will suffice to show that every $p\in(a-\delta,a+\delta)$ is an element of $\{x\in\R\mid|x-a|<\delta\}$ and vice versa.\par
        Suppose first that $p\in(a-\delta,a+\delta)$. Then by Equations \ref{eqn:8.1}, $a-\delta<p$ and $p<a+\delta$. It follows by consecutive applications of Definition \ref{dfn:7.21} from the former condition that $-\delta<p-a$, and from the latter condition that $p-a<\delta$. Since $-\delta<p-a<\delta$, the lemma asserts that $|p-a|<\delta$. Therefore, $p\in\{x\in\R\mid|x-a|<\delta\}$.\par
        Now suppose that $p\in\{x\in\R\mid|x-a|<\delta\}$. Then $|p-a|<\delta$. Thus, by the lemma, $-\delta<p-a$ and $p-a<\delta$. It follows by consecutive applications of Definition \ref{dfn:7.21} from the former condition that $a-\delta<p$, and from the latter condition that $p<a+\delta$. Therefore, since $a-\delta<p<a+\delta$, we have that $p\in(a-\delta,a+\delta)$.
    \end{proof}
\end{exercise}




\end{document}